##### 三角函数微积分
- 三角函数求导
	- $\displaystyle\frac{{\rm d}}{{\rm d}x}\sin(x)=\cos(x)$
		- $=\displaystyle\lim_{h\rightarrow0}\frac{\sin(x+h)-\sin(x)}{h}$
		- $=\displaystyle\lim_{h\rightarrow0}\frac{\sin(x)\cos(h)+\cos(x)\sin(h)-\sin(x)}{h}$
		- $=\displaystyle\lim_{h\rightarrow0}(\sin(x)(\frac{\cos(h)-1}{h})+\cos(x)(\frac{\sin(h)}{h}))$
		- $=\sin(x)\times0+\cos\times1=\cos(x)$
	- $\displaystyle\frac{{\rm d}}{{\rm d}x}\cos(x)=-\sin(x)$
		- $=\displaystyle\lim_{h\rightarrow0}\frac{\cos(x+h)-\cos(x)}{h}$
		- $=\displaystyle\lim_{h\rightarrow0}\frac{\cos(x)\cos(h)-\sin(x)\sin(h)-\cos(x)}{h}$
		- $=\displaystyle\lim_{h\rightarrow0}(\cos(x)(\frac{\cos(h)-1}{h})-\sin(x)(\frac{\sin(h)}{h}))$
		- $=\cos(x)\times0-\sin\times1=-\sin(x)$
	- $\displaystyle\frac{{\rm d}}{{\rm d}x}\tan(x)=\sec^2(x)$
		- $\displaystyle=\frac{{\rm d}}{{\rm d}x}\frac{\sin(x)}{\cos(x)}=\frac{\cos(x)\cos(x)+\sin(x)\sin(x)}{\cos^2(x)}$
		- $\displaystyle=\frac{1}{\cos^2(x)}=\sec^2(x)$
	- $\displaystyle\frac{{\rm d}}{{\rm d}x}\sec(x)=\sec(x)\tan(x)$
		- $\displaystyle=\frac{{\rm d}}{{\rm d}x}\frac{1}{cos(x)}=\frac{{\rm d}}{{\rm d}u}\frac{1}{u}\cdot\frac{{\rm d}}{{\rm d}x}\cos(x)$
		- $\displaystyle=(-\frac{1}{u^2})(-\sin(x))=\frac{\sin(x)}{\cos^2(x)}=\sec(x)\tan(x)$
	- $\displaystyle\frac{{\rm d}}{{\rm d}x}\csc(x)=-\csc(x)\cot(x)$
		- $\displaystyle=\frac{{\rm d}}{{\rm d}x}\frac{1}{sin(x)}=\frac{{\rm d}}{{\rm d}u}\frac{1}{u}\cdot\frac{{\rm d}}{{\rm d}x}\sin(x)$
		- $\displaystyle=(-\frac{1}{u^2})(\cos(x))=-\frac{\cos(x)}{\sin^2(x)}=-\csc(x)\cot(x)$
	- $\displaystyle\frac{{\rm d}}{{\rm d}x}\cot(x)=-\csc^2(x)$
		- $\displaystyle=\frac{{\rm d}}{{\rm d}x}\frac{\cos(x)}{\sin(x)}=\frac{-\sin(x)\sin(x)-\cos(x)\cos(x)}{\sin^2(x)}$
		- $\displaystyle=\frac{1}{\sin^2(x)}=-\csc^2(x)$
- 三角函数积分
	- $\displaystyle\int \cos x{\rm d}x=\sin x+C$
	- $\displaystyle\int \sin x{\rm d}x=-\cos x+C$
	- $\displaystyle\int {\frac{1}{\cos^2x}} {\rm d}x=\displaystyle\int {\sec^2} {\rm d}x=\tan x+C$
	- $\displaystyle\int {\frac{1}{\sin^2x}} {\rm d}x=\displaystyle\int {\csc^2} {\rm d}x=-\cot x+C$
	- $\displaystyle\int \sec x \tan x{\rm d}x=\sec x+C$
	- $\displaystyle\int \csc x \cot x{\rm d}x=-\csc x+C$

