##### 伴随映射
- 伴随映射 [[伴随映射的矩阵|矩阵]]
	- **伴随映射** $T^*:W\rightarrow V$ 是定义在[[内积空间]]上的[[线性变换]], 满足保持[[内积]]不变, 即使得对任意 $\mathbf{v}\in V$, $\mathbf{w}\in W$ 有 $\langle T(\mathbf{v}),\mathbf{w}\rangle=\langle\mathbf{v},T^*(\mathbf{w})\rangle$
		- $T(\mathbf{v})=A\mathbf{v}$, $T^*(\mathbf{w})=A^*\mathbf{w}$

$$\begin{array}{ccc} V & \xleftrightharpoons[T^*]{T} & W \\ \updownarrow & & \updownarrow \\ V' & \xleftarrow{T'} & W' \end{array}$$


>[!example]- 伴随映射
>- $T \in L(\mathbb{R}^3,\mathbb{R}^2)$, $T(x_1,x_2,x_3)=(x_2+3x_3,2x_1)$
>	- 设 $(x_1,x_2,x_3)\in\mathbb{R}^3$, $(y_1,y_2)\in\mathbb{R}^2$
>		- $\begin{align}\langle T(x_1,x_2,x_3),(y_1,y_2)\rangle &= \langle T(x_2+3x_3,2x_1),(y_1,y_2)\rangle\\&=x_2y_1+3x_3y_1+2x_1y_2\\&=\langle(x_1,x_2,x_3),(2y_2,y_1,3y_1)\rangle\end{align}$
>		- $T^*(y_1,y_2)=(2y_2,y_1,3y_1)$
>	- 设 ${R}^3$, ${R}^2$ 都为标准正交基
>		- $M_T = \begin{bmatrix} 0 & 1 & 3 \\ 2 & 0 & 0 \end{bmatrix}$
>		- $M_{T^*} = \begin{bmatrix} 0 & 2 \\ 1 & 0 \\ 3 & 0 \end{bmatrix}$
>		- $M_{T^*}=M_{T}^*$

