##### 反函数微积分
- 反函数求导
	- $\displaystyle \frac{{\rm d}y}{{\rm d}x}=\frac{1}{f'(y)}$
		- 求导: $\displaystyle x=f(y)$
		- $\displaystyle \frac{{\rm d}}{{\rm d}x}(x)=\frac{{\rm d}}{{\rm d}x}(f(y))$
		- $\displaystyle 1=\frac{{\rm d}u}{{\rm d}y}\frac{{\rm d}y}{{\rm d}x}=f'(y)\frac{{\rm d}y}{{\rm d}x}$
		- $\displaystyle \frac{{\rm d}y}{{\rm d}x}=\frac{1}{f'(y)}$

>[!example]- 反函数求导
>- $f(x)=x^3$
>	- 反函数 $y=f^{-1}(x)=x^{\frac{1}{3}}$
>	- $\displaystyle \frac{{\rm d}y}{{\rm d}x}=\frac{1}{f'(y)}=\frac{1}{3y^2} =\frac{1}{3(x^{\frac{1}{3}})^2}=\frac{1}{3x^{\frac{2}{3}}}$
