##### 复合函数微积分
- 复合函数求导
	- $\displaystyle f'(g(x))=f'(g(x))g'(x)$
	- $\displaystyle\frac{{\rm d}y}{{\rm d}x}=\frac{{\rm d}y}{{\rm d}u}\frac{{\rm d}u}{{\rm d}x}$
- 复合函数微分
	- $y=f(u)$, $u=g(x)$, $y=f(g(x))$
	- ${\rm d}(f(u))=f'(u){\rm d}x=f'(u)g'(x){\rm d}x=f'(u){\rm d}u$

>[!example]- 复合函数求导
>- $\displaystyle f(x)=\ln(2x+5)$
>	- $\displaystyle g(x)=2x+5$
>	- $\displaystyle f'[g(x)]=f'[g(x)]g'(x)=\frac{2}{2x+5}$
>- $\displaystyle f(x)=(x^2+1)^{99}$ 
>	- $\displaystyle y=u^{99},u=x^2+1$
>	- $\displaystyle\frac{{\rm d}y}{{\rm d}x}=\frac{{\rm d}y}{{\rm d}u}\frac{{\rm d}u}{{\rm d}x}=99u^{98}\cdot 2x=198(x^2+1)^{98}$
