##### 复数基础运算
- 复数基础运算
	- 加法 $z_1+z_2=(x_1+x_2,y_1+y_2)$
		- $z_1 + 0 = z_1$
		- $-z_1=(-x_1,-y_1)$
		- $z_1 + z_2 = z_2 + z_1$ 
		- $(z_1 + z_2) + z_3 = z_1 + (z_2 + z_3)$ 
	- 减法 $z_1-z_2=z_1+(-z_2)$
	- 乘法 $z_1z_2=(x_1x_2-y_1y_2,y_1x_2+x_1y_2)$ 
		- $z_1\cdot 1=z_1$
		- $z_1\cdot 0=0$
		- $\displaystyle z_1^{-1}=(\frac{x_1}{x_1^2+y_1^2},\frac{-y_1}{x_1^2+y_1^2})$
		- $z_1z_2 = z_2z_1$
		- $(z_1z_2)z_3 = z_1(z_2z_3)$
		- $z_3(z_1 + z_2)=z_3z_1+z_3z_2$
	- 除法 $\displaystyle\frac{z_1}{z_2}=z_1z_1^{-1}$

