##### 导数基础运算
- 导数基础运算
	- 和差
		- $\displaystyle[f(x)\pm g(x)]'=f'(x)\pm g'(x)$
		- $\displaystyle\frac{\text{d}(f\pm g)}{\text{d}x}=\frac{\text{d}f}{\text{d}x}\pm\frac{\text{d}g}{\text{d}x}$
		 - ${\rm d}(u\pm v)={\rm d}u\pm{\rm d}v$
	- 乘积
		- $\displaystyle[f(x)g(x)]'=f'(x)g(x)+f(x)g'(x)$
		- $\displaystyle\frac{\text{d}(fg)}{\text{d}x}=g\frac{\text{d}f}{\text{d}x}+f\frac{\text{d}g}{\text{d}x}$
		- ${\rm d}(uv)=v{\rm d}u+u{\rm d}v$
	- 除法
		- $\displaystyle[\frac{f(x)}{g(x)}]'=\frac{f'(x)g(x)-f(x)g'(x)}{g^2(x)}$
		- $\displaystyle\frac{\text{d}(\frac{f}{g})}{\text{d}x}=\frac{g\frac{\text{d}f}{\text{d}x}-f\frac{\text{d}g}{\text{d}x}}{g^2}$
		- $\displaystyle{\rm d}(\frac{u}{v})=\frac{v{\rm d}u-u{\rm d}v}{v^2}$
	- 复合函数求导 (链式求导)
		- $\displaystyle f'[g(x)]=f'[g(x)]g'(x)$
		- $\displaystyle \frac{{\rm d}f[g(x)]}{{\rm d}x}=\frac{{\rm d}f(g)}{{\rm d}g}\frac{{\rm d}g}{{\rm d}x}$
		- ${\rm d}(f(u))=f'(u)g'(x){\rm d}x=f'(u){\rm d}u$
	- 反函数求导
		- $\displaystyle \frac{{\rm d}y}{{\rm d}x}=\frac{1}{f'(y)}$
			- 求导: $\displaystyle x=f(y)$
			- $\displaystyle \frac{{\rm d}}{{\rm d}x}(x)=\frac{{\rm d}}{{\rm d}x}(f(y))$
			- $\displaystyle 1=\frac{{\rm d}u}{{\rm d}y}\frac{{\rm d}y}{{\rm d}x}=f'(y)\frac{{\rm d}y}{{\rm d}x}$
			- $\displaystyle \frac{{\rm d}y}{{\rm d}x}=\frac{1}{f'(y)}$
	- 取对数求导
		- $\displaystyle y=f(x)^{g(x)}$
		- $\ln(y)=g(x)\ln(f(x))$
		- $\displaystyle\frac{1}{y}\frac{{\rm d}y}{{\rm d}x}=\frac{{\rm d}}{{\rm d}x}...$
	- 隐函数求导
		- 对方程两边一切同时求导并化简

>[!example]- 复合函数求导
>- $\displaystyle f(x)=\ln(2x+5)$
>	- $\displaystyle g(x)=2x+5$
>	- $\displaystyle f'[g(x)]=f'[g(x)]g'(x)=\frac{2}{2x+5}$
>- $\displaystyle f(x)=(x^2+1)^{99}$ 
>	- $\displaystyle y=u^{99},u=x^2+1$
>	- $\displaystyle\frac{{\rm d}y}{{\rm d}x}=\frac{{\rm d}y}{{\rm d}u}\frac{{\rm d}u}{{\rm d}x}=99u^{98}\cdot 2x=198(x^2+1)^{98}$

>[!example]- 隐函数求导
>- $y=\cos(x+y)$
>	- $\displaystyle \frac{{\rm d}}{{\rm d}x}y=\frac{{\rm d}}{{\rm d}x}\cos(x+y)$
>	- 链式求导 $\displaystyle \frac{{\rm d}y}{{\rm d}x}=-(1+\frac{{\rm d}y}{{\rm d}x})\sin(x+y)$
>	- $\displaystyle \frac{{\rm d}y}{{\rm d}x}=\frac{-\sin(x+y)}{1+\sin(x+y)}$

>[!example]- 反函数求导 
>- $f(x)=x^3$
>	- 反函数 $y=f^{-1}(x)=x^{\frac{1}{3}}$
>	- $\displaystyle \frac{{\rm d}y}{{\rm d}x}=\frac{1}{f'(y)}=\frac{1}{3y^2} =\frac{1}{3(x^{\frac{1}{3}})^2}=\frac{1}{3x^{\frac{2}{3}}}$