##### 泰勒展开实例
- 泰勒展开实例
	- 函数在 $x=0$ 的[[泰勒级数|泰勒展开式]]
		- $\displaystyle e^x$, $x\in(-\infty,+\infty)$
			- $\displaystyle 1+x+\frac{x^2}{2!}+...+\frac{x^n}{n!}+...=\sum^{\infty}_{n=0}\frac{x^n}{n!}$
		- $\displaystyle\frac{1}{1+x}$, $x\in(-1,1)$
			- $\displaystyle1-x+x^2+...+(-1)^nx^n+...= \sum^{\infty}_{n=0} (-1)^nx^n$
		- $\displaystyle\frac{1}{1-x}$, $x\in(-1,1)$
			- $\displaystyle1+x+x^2+...+x^n+...= \sum^{\infty}_{n=0} x^n$
		- $\displaystyle \ln{(1+x)}$, $x\in(-1,1]$
			- $\displaystyle x-\frac{x^2}{2}+\frac{x^3}{3}+...+(-1)^{n-1}\frac{x^n}{n}+... = \sum^{\infty}_{n=1} (-1)^{n-1}\frac{x^n}{n}$
		- $\displaystyle \sin{x}$, $x\in(-\infty,+\infty)$
			- $\displaystyle x-\frac{x^3}{3!}+\frac{x^5}{5!}+...+(-1)^n\frac{x^{2n+1}}{(2n+1)!} = \sum^{\infty}_{n=0} (-1)^n\frac{x^{2n+1}}{(2n+1)!}$
		- $\displaystyle \cos{x}$, $x\in(-\infty,+\infty)$
			- $\displaystyle x-\frac{x^2}{2!}+\frac{x^4}{4!}+...+(-1)^n\frac{x^{2n}}{(2n)!}= \sum^{\infty}_{n=0} (-1)^n\frac{x^{2n}}{(2n)!}$


